reduce scope

authoring/knapsack.dfy
@@ -1,29 +1,109 @@
-module KS {
+include "../authoring/seq.dfy"
+
+module SixSeventeen {
+    import Seq = Seq
+
     class Obj {
         var weight: int;
         var value: int;
     }
 
-    lemma sums(objs: set<Obj>) returns (totWeight: int, totValue: int)
+    function totalWeight(s: seq<Obj>): int
+    requires |s|>0
+    decreases |s|
+    reads s
     {
-        var objs' :set<Obj> := objs;
-        while objs' != {}
-        decreases objs'
-        {
-            var t :| t in objs';
-            totWeight := totWeight + t.weight;
-            totValue := totValue + t.value;
-            objs' := objs' - {t};
-        }
+        if |s| == 1 then s[0].weight else
+        s[0].weight + totalWeight(s[1..])
     }
 
+    function method weightsLT(s: seq<Obj>, weight: int): seq<Obj>
+    requires |s|>0
+    decreases |s|
+    reads s
+    {
+        if |s| == 1 then if s[0].weight <= weight then [s[0]] else []
+        else if s[0].weight <= weight then [s[0]] + weightsLT(s[1..], weight)
+        else weightsLT(s[1..], weight)
+    }
+
+    /**
+     * The sum of weights in the optimum subset
+     * is no more than the knapsack capacity.
+     */
     predicate a1(totWeight: int, capacity: nat)
     {
         totWeight <= capacity
     }
 
-    lemma ks(objs: set<Obj>, capacity: nat) returns (so: set<Obj>, totWeight: int)
-    ensures so <= objs
-            && a1(totWeight, capacity)
-    {}
+    /**
+     * This helps rule out trivial corner cases. 
+     * Total weight is the sum of all object weights before algorithm begins.
+     * See: https://pdfs.semanticscholar.org/8bc5/7f44bdd880a385b7c1338293ea4183f930ea.pdf
+     */
+     predicate a5(objs: seq<Obj>, totWeight: int, capacity: nat)
+     reads objs
+     {
+         totWeight > capacity
+         && forall o :: o in objs ==> o.weight <= capacity
+     }
+
+    /**
+     * Optimum sum of values in the set.
+     */
+    predicate a2(maxVal: int, objs: seq<Obj>)
+    {
+        false
+        //forall i :: i <= objs ==> maxVal >= 
+    }
+
+    /**
+     * Knapsack type 2: with repetitions, i.e., unlimited
+     * copies of each object.
+     */
+    method coinsDP(objs: seq<Obj>, s: seq<int>, capacity: nat) returns (maxVal: int)
+    requires |s| == capacity+1 > 0 && s[0] == 0
+    requires capacity > 1
+    requires |objs| > 0
+    requires a5(objs, totalWeight(objs), capacity)
+    ensures a2(maxVal, objs)
+    {
+        var se := s;
+        var i := 1;
+
+        while i < capacity
+        invariant capacity == capacity
+        invariant |se| == capacity+1
+        invariant 0 <= i <= capacity
+        decreases capacity-i
+        {
+            var objslt := weightsLT(objs, i);
+            assert |objslt| <= |objs|;
+            assert multiset(objslt) <= multiset(objs);
+            var j := 0;
+            var subOpt := 0;
+
+            while j < |objslt|-1
+            invariant 0 <= j <= |objslt|-1
+            invariant forall o :: o in objslt ==> o.weight <= i
+            decreases |objslt|-j
+            {
+                var nw := i-objslt[j].weight;
+                var nw' := i-objslt[j+1].weight;
+                if se[nw] + objslt[j].value <= se[nw'] + objslt[j+1].value
+                {
+                    subOpt := se[nw']+objslt[j+1].value;
+                } else { subOpt := se[nw]+objslt[j].value; }
+
+                j := j+1;
+            }
+
+            assert |se| == capacity+1;
+            assert i <= |se| == capacity+1;
+
+            if j >= 1 {se := se[i := subOpt]; }
+            j := 0;
+            i := i+1;
+        }
+    }
 }
